Bdd/Count.lean
@@ -18,7 +18,7 @@ private def my_vector_equiv_vector : List.Vector α n ≃ Vector α n where
   toFun     := fun l ↦ ⟨l.toList.toArray, .trans List.size_toArray   (List.Vector.toList_length _)⟩
   invFun    := fun v ↦ ⟨v.toList,         .trans Array.length_toList (Vector.size_toArray       _)⟩
   left_inv  := fun x ↦ (by simp)
-  right_inv := fun x ↦ (by simp)
+  right_inv := fun x ↦ (by simp; try rfl)
 
 private instance instVectorFintype [Fintype α] {n : ℕ} : Fintype (Vector α n) := Fintype.ofEquiv (List.Vector α n) my_vector_equiv_vector
 
