Bdd/Lift.lean
@@ -53,8 +53,8 @@ private lemma lift_preserves_MayPrecede {h : n ≤ n'} {B : Bdd n m} {p q : Poin
       | terminal _ =>
         apply Pointer.MayPrecede_node_terminal
       | node j' =>
-        simp only [Pointer.MayPrecede, Nat.succ_eq_add_one, lift, Pointer.toVar_node_eq, Fin.getElem_fin] at hm
-        apply (Fin.natCast_lt_natCast (by omega) (by omega)).mp at hm
+        simp only [Pointer.MayPrecede, Nat.succ_eq_add_one, Pointer.toVar, lift, Fin.getElem_fin,
+          Vector.getElem_map, Fin.mk_lt_mk, Fin.val_fin_lt] at hm
         simp only [Pointer.MayPrecede, Nat.succ_eq_add_one, Pointer.toVar_node_eq, Fin.getElem_fin]
         aesop
   · intro hm
@@ -69,8 +69,7 @@ private lemma lift_preserves_MayPrecede {h : n ≤ n'} {B : Bdd n m} {p q : Poin
       | node j' =>
         simp only [Pointer.MayPrecede, Nat.succ_eq_add_one, Pointer.toVar_node_eq, Fin.getElem_fin] at hm
         simp only [Pointer.MayPrecede, Nat.succ_eq_add_one, lift, Pointer.toVar_node_eq, Fin.getElem_fin]
-        simp_all only [Fin.coe_eq_castSucc, Fin.castSucc_lt_castSucc_iff, Vector.getElem_map]
-        refine (Fin.natCast_lt_natCast ?_ ?_).mpr ?_ <;> omega
+        simp_all [Fin.coe_eq_castSucc, Fin.castSucc_lt_castSucc_iff, Vector.getElem_map, Pointer.toVar]
 
 private lemma lift_preserves_RelevantEdge {h : n ≤ n'} {B : Bdd n m} {p q : Pointer m} :
     ( ∃ (hp : Pointer.Reachable (lift h B).heap (lift h B).root p)
